\documentclass[12pt,english]{article}
\usepackage{geometry}
\usepackage{float}
\usepackage{caption}
\geometry{verbose,tmargin=3cm,bmargin=3cm,lmargin=3cm,rmargin=3cm}
\usepackage{amsmath}
\usepackage{amssymb}
\usepackage{amsthm}
\usepackage{verbatim}
\usepackage{adjustbox}
\usepackage{hyperref}
\usepackage{graphicx}
\usepackage{setspace}
\usepackage{changepage}
\usepackage{enumitem}
\setlist{nolistsep}
\onehalfspacing
\usepackage{babel}
\newcommand{\expec}{\ensuremath{\mathbb E}}
\begin{document}
\begin{center}
{\Large{}Section 2: Random variables (solutions)}
\par\end{center}{\Large \par}

\begin{center}
ARE 210
\par\end{center}

\begin{center}
September 5, 2017
\par\end{center}

\noindent
1) \textbf{Probability of complement}: Show that $P(A^{c}) = 1 - P(A)$.
\vspace{1em}

By the law of total probability, $P(A^{c}) + P(A) = 1$. Subtracting yields $P(A^{c}) = 1 - P(A)$.

\vspace{1em}
\noindent
2) \textbf{Conditional Bayes' Theorem}: Show that $P(A | B, C) = \frac{P(A, B | C)}{P(B | C)}$
\vspace{1em}

\begin{align*}
P(A | B, C) & = \frac{P(A, B, C)}{P(B, C)} \\
& = \frac{P(A, B | C) P(C)}{P(B | C) P(C)} \\
& = \frac{P(A, B |C)}{P(B | C)}
\end{align*}

\vspace{1em}
\noindent
3) \textbf{Mixed random variables}: Let $(X_{1}, X_{2})$ be random variables with joint distribution $F$. How would you calculate the marginal distribution of $X_{1}$?
\vspace{1em}

$$ F_{1}(x_{1}) = \lim_{x_{2} \to \infty} F(x_{1}, x_{2}) $$

$$ f_{1}(x_{1}) = \int_{-\infty}^{\infty} f(x_{1}, x_{2}) dx_{2} $$\

\vspace{1em}
\noindent
4) \textbf{Independence and densities}: Let $X_{1}, X_{2}$ be independent continuous random variables. Show that their joint density is equal to the product of their marginal densities, and assume for simplicity that each has a continuous marginal density.

First, their joint distribution $F(x_{1}, x_{2}) = F_{1}(x_{1}) F_{2}(x_{2})$. Substituting for the definitions of the CDF in terms of the density and merging the integration yields $F(x_{1}, x_{2}) = \int_{-\infty}^{x_{1}} \int_{-\infty}^{x_{2}} f_{1}(\widetilde{x_{1}}) f_{2}(\widetilde{x_{2}}) d\widetilde{x_{2}} d\widetilde{x_{1}}$, which implies that $f(x_{1}, x_{2}) = f_{1}(x_{1}) f_{2}(x_{2})$.

\vspace{1em}
\noindent
5) \textbf{Distribution practice}: Let $X_{1}, X_{2}$ be standard normal random variables, each with density $f(x) = \frac{1}{\sqrt{2\pi}} e^{-\frac{x^{2}}{2}}$. \\
a) What is the joint distribution $F$ of $X_{1}$ and $X_{2}$? What is the joint density $f$? \\

$$ F(x_{1}, x_{2}) = \Phi(x_{1}) \Phi(x_{2}) =  \frac{1}{2\pi} \int_{-\infty}^{x_{1}} \int_{-\infty}^{x_{2}} \exp \left\{ -\frac{\widetilde{x_{1}}^{2} + \widetilde{x_{2}}^{2}}{2} \right\} d\widetilde{x_{2}} d\widetilde{x_{1}} $$

$$ f(x_{1}, x_{2}) = \phi(x_{1}) \phi(x_{2}) = \frac{1}{2\pi} \exp \left\{ -\frac{\widetilde{x_{1}}^{2} + \widetilde{x_{2}}^{2}}{2} \right\} $$

\vspace{1em}
\noindent
b) What is the distribution $F_{Y}$ of $Y = X_{1} + X_{2}$? What is the density $f_{Y}$? \\

Let $\phi$ be the standard normal density and $\Phi$ be the standard normal CDF.

\begin{align*}
F_{Y}(y) & = \int_{-\infty}^{\infty} \int_{-\infty}^{y - x_{1}} \phi(x_{1}) \phi(x_{2}) dx_{2} dx_{1} \\
& = \int_{-\infty}^{\infty} \phi(x_{1}) \Phi(y - x_{1}) dx_{1} \\
\end{align*}

Differentiating with respect to $y$ yields

\begin{align*}
f_{Y}(y) & = \int_{-\infty}^{\infty} \phi(x_{1}) \phi(y - x_{1}) dx_{1} \\
& = \frac{1}{2\pi} \int_{-\infty}^{\infty} \exp \left\{ -\frac{x_{1}^{2}}{2}\right\} \exp \left\{ -\frac{(y - x_{1})^{2}}{2}\right\} dx_{1} \\
& = \frac{1}{2\sqrt{\pi}} \exp \left\{ -\frac{y^{2}}{4} \right\} \int_{-\infty}^{\infty} \frac{1}{\sqrt{\pi}} \exp \left\{ - \left(x_{1} - \frac{y}{2} \right)^{2}\right\} dx_{1} \\
& = \frac{1}{2\sqrt{\pi}} \exp \left\{ -\frac{y^{2}}{4} \right\}
\end{align*}

Integrating again yields

\begin{align*}
F_{Y}(y) = \frac{1}{2\sqrt{\pi}} \int_{-\infty}^{y} \exp \left\{ -\frac{\widetilde{y}^{2}}{4} \right\} d \widetilde{y}
\end{align*}

\begin{comment}
\vspace{1em}
\noindent
c) What is the joint distribution $G$ of $X_{1}$ and $Y$? What is the joint density $g$? \\

\begin{align*}
G(x_{1}, y) & = F(x_{1}, y - x_{1}) \\
& = \Phi(x_{1}) \Phi(y - x_{1})
\end{align*}

\begin{align*}
g(x_{1}, y) & = \frac{\partial}{\partial x_{1}} \frac{\partial}{\partial y} G(x_{1}, y) \\
& = \frac{\partial}{\partial x_{1}} \Phi(x_{1}) \phi(y - x_{1}) \\
& = \phi(x_{1}) \phi(y - x_{1}) - \Phi(x_{1}) \phi'(y - x_{1})
\end{align*}
\end{comment}
\end{document}